Capless/Store.lean
@@ -3,6 +3,7 @@ import Capless.Type
 import Capless.CaptureSet
 import Capless.Context
 import Capless.Typing
+import Capless.ReachSet
 
 /-!
 # Evaluation States
@@ -168,33 +169,6 @@ theorem Cont.HasLabel.has_intercept (hl : HasLabel cont l tail) : ∃ h tail', H
     cases b0
     . exists .some h0, cont; apply HasIntercept.here_intercept hl hd;
     . exists h, tail; apply! HasIntercept.there_intercept
-
-/-- Computes the reach set of a capture set. The reach set should only consist of capture variables and -/
-inductive ReachSet : Context n m k -> CaptureSet n k -> CaptureSet n k -> Prop where
-| empty : ReachSet Γ .empty .empty
-| union :
-  ReachSet Γ C1 R1 ->
-  ReachSet Γ C2 R2 ->
-  ReachSet Γ (C1 ∪ C2) (R1 ∪ R2)
-| var :
-  Context.Bound Γ x (S^C) ->
-  ReachSet Γ (C.proj L) R ->
-  ReachSet Γ {x=x|L} R
-| cinstr :
-  Context.CBound Γ c (CBinding.inst C) ->
-  ReachSet Γ (C.proj L) R ->
-  ReachSet Γ {c=c|L} R
-| cbound :
-  Context.CBound Γ c (CBinding.bound (CBound.upper C)) ->
-  ReachSet Γ (C.proj L) R ->
-  ReachSet Γ {c=c|L} R
-| ckind :
-  Context.CBound Γ c (CBinding.bound (CBound.kind K)) ->
-  ReachSet Γ {c=c|L} {c=c|K.intersect L}
-| label :
-  Context.LBound Γ x c S ->
-  ReachSet Γ {x=x|L} {x=x|(Kind.classifier c).intersect L}
-| absurd : K.IsEmpty -> ReachSet Γ (.singleton s K) {}
 
 /-- Checks whether a capture set is well-scoped under a context and a continuation stack.
  -- A capture set is well-scoped if any label transitively reachable from it is in the scope of the continuation stack (via `Cont.HasLabel`).
