Capless/ReachSet.lean
@@ -1,0 +1,33 @@
+import Capless.CaptureSet
+import Capless.Context
+
+namespace Capless
+
+/-- Computes the reach set of a capture set. The reach set should only consist of capture variables and -/
+inductive ReachSet : Context n m k -> CaptureSet n k -> CaptureSet n k -> Prop where
+| empty : ReachSet Γ .empty .empty
+| union :
+  ReachSet Γ C1 R1 ->
+  ReachSet Γ C2 R2 ->
+  ReachSet Γ (C1 ∪ C2) (R1 ∪ R2)
+| var :
+  Context.Bound Γ x (S^C) ->
+  ReachSet Γ (C.proj L) R ->
+  ReachSet Γ {x=x|L} R
+| cinstr :
+  Context.CBound Γ c (CBinding.inst C) ->
+  ReachSet Γ (C.proj L) R ->
+  ReachSet Γ {c=c|L} R
+| cbound :
+  Context.CBound Γ c (CBinding.bound (CBound.upper C)) ->
+  ReachSet Γ (C.proj L) R ->
+  ReachSet Γ {c=c|L} R
+| ckind :
+  Context.CBound Γ c (CBinding.bound (CBound.kind K)) ->
+  ReachSet Γ {c=c|L} {c=c|K.intersect L}
+| label :
+  Context.LBound Γ x c S ->
+  ReachSet Γ {x=x|L} {x=x|(Kind.classifier c).intersect L}
+| absurd : K.IsEmpty -> ReachSet Γ (.singleton s K) {}
+
+end Capless
