Capless/Weakening/TypedCont/Capture.lean
@@ -70,38 +70,42 @@ theorem Cont.HasLabel.cweaken
   case there_label => simp [Cont.cweaken]; apply there_label; aesop
   case there_intercept => simp [Cont.cweaken]; apply there_intercept; aesop
 
+theorem ReachSet.cweaken
+  (hr : ReachSet Γ C R)
+  : ReachSet (Γ.cvar b) C.cweaken R.cweaken := by
+  induction hr
+  case empty => constructor
+  case union ha hb => apply! union
+  case var hb hr ih =>
+    have hb1 := hb.there_cvar (b:=b)
+    apply var hb1
+    rw [← CaptureSet.proj_crename]; exact ih
+  case cinstr hb hr ih =>
+    have hb1 := hb.there_cvar (b':=b)
+    apply cinstr hb1
+    rw [← CaptureSet.proj_crename]; exact ih
+  case cbound hb hr ih =>
+    have hb1 := hb.there_cvar (b':=b)
+    apply cbound hb1
+    rw [← CaptureSet.proj_crename]; exact ih
+  case ckind hb =>
+    have hb1 := hb.there_cvar (b':=b)
+    apply ckind hb1
+  case label hb =>
+    have hb1 := hb.there_cvar (b:=b)
+    apply label hb1
+  case absurd he => apply! absurd
+
 theorem WellScoped.cweaken
   (h : WellScoped Γ E Ct) :
   WellScoped (Γ.cvar b) E.cweaken Ct.cweaken := by
   induction h
-  case empty => constructor
-  case union ih1 ih2 => apply union <;> aesop
-  case singleton hb _ ih =>
-    apply singleton
-    { have hb1 := Context.Bound.there_cvar (b := b) hb
-      simp [CType.cweaken, CType.crename] at hb1
-      exact hb1 }
-    { rw [← CaptureSet.proj_crename]; exact ih }
-  case csingleton hb _ ih =>
-    apply csingleton
-    { have hb1 := Context.CBound.there_cvar (b' := b) hb
-      simp [CType.cweaken, CType.crename] at hb1
-      exact hb1 }
-    { rw [← CaptureSet.proj_cweaken]; exact ih }
-  case cbound hb _ ih =>
-    apply cbound
-    { have hb1 := Context.CBound.there_cvar (b' := b) hb
-      simp [CType.cweaken, CType.crename] at hb1
-      exact hb1 }
-    { rw [← CaptureSet.proj_crename]; exact ih }
-  case ckind hb => apply ckind hb.there_cvar
-  case label hb hs =>
-    apply label
-    { have hb1 := Context.LBound.there_cvar (b := b) hb
-      simp [CType.cweaken, CType.crename] at hb1
-      exact hb1 }
-    { apply hs.cweaken }
+  case empty => apply! empty
+  case union ha hb => apply! union
+  case ckind hb => apply! ckind hb.there_cvar
+  case label hb hl => apply label hb.there_cvar hl.cweaken
   case label_disj hb hd => apply! label_disj hb.there_cvar
+  case absurd => apply! absurd
 
 theorem TypedCont.cweaken
   (h : TypedCont Γ Cin E t E' Ct) :
