Capless/Weakening/TypedCont/Term.lean
@@ -73,38 +73,77 @@ theorem Cont.HasLabel.weaken
   case there_intercept ih =>
     apply there_intercept; trivial
 
+-- theorem WellScoped.weaken
+--   (h : WellScoped Γ cont Ct) :
+--   WellScoped (Γ.var T) cont.weaken Ct.weaken := by
+--   induction h
+--   case empty => simp [CaptureSet.weaken]; constructor
+--   case union ih1 ih2 =>
+--     simp [CaptureSet.weaken] at *
+--     apply union <;> aesop
+--   case singleton hb _ ih =>
+--     apply singleton
+--     { simp [FinFun.weaken]
+--       have hb1 := Context.Bound.there_var (E':=T) hb
+--       simp [CType.weaken, CType.rename] at hb1
+--       exact hb1 }
+--     { rw [← CaptureSet.proj_rename]; exact ih }
+--   case csingleton hb _ ih =>
+--     apply csingleton
+--     { have hb1 := Context.CBound.there_var (E:=T) hb
+--       exact hb1 }
+--     { rw [← CaptureSet.proj_rename]; exact ih }
+--   case cbound hb _ ih =>
+--     apply cbound
+--     { have hb1 := Context.CBound.there_var (E:=T) hb
+--       exact hb1 }
+--     { rw [← CaptureSet.proj_rename]; exact ih }
+--   case ckind hb => apply ckind hb.there_var
+--   case label hb hs =>
+--     apply label
+--     { have hb1 := Context.LBound.there_var (E:=T) hb
+--       exact hb1 }
+--     { apply hs.weaken }
+--   case label_disj hb hd => apply label_disj hb.there_var hd
+
+theorem ReachSet.weaken
+  (hr : ReachSet Γ C R)
+  : ReachSet (Γ.var T) C.weaken R.weaken := by
+  induction hr
+  case empty => constructor
+  case union ha hb => apply! union
+  case var hb hr ih =>
+    have hb1 := hb.there_var (E':=T)
+    simp [CType.weaken, CType.rename] at hb1
+    apply var hb1
+    rw [← CaptureSet.proj_rename]; exact ih
+  case cinstr hb hr ih =>
+    have hb1 := hb.there_var (E:=T)
+    apply cinstr hb1
+    rw [← CaptureSet.proj_rename]; exact ih
+  case cbound hb hr ih =>
+    have hb1 := hb.there_var (E:=T)
+    apply cbound hb1
+    rw [← CaptureSet.proj_rename]; exact ih
+  case ckind hb =>
+    have hb1 := hb.there_var (E:=T)
+    apply ckind hb1
+  case label hb =>
+    have hb1 := hb.there_var (E:=T)
+    apply label hb1
+  case absurd he => apply! absurd
+
 theorem WellScoped.weaken
   (h : WellScoped Γ cont Ct) :
   WellScoped (Γ.var T) cont.weaken Ct.weaken := by
   induction h
-  case empty => simp [CaptureSet.weaken]; constructor
-  case union ih1 ih2 =>
-    simp [CaptureSet.weaken] at *
-    apply union <;> aesop
-  case singleton hb _ ih =>
-    apply singleton
-    { simp [FinFun.weaken]
-      have hb1 := Context.Bound.there_var (E':=T) hb
-      simp [CType.weaken, CType.rename] at hb1
-      exact hb1 }
-    { rw [← CaptureSet.proj_rename]; exact ih }
-  case csingleton hb _ ih =>
-    apply csingleton
-    { have hb1 := Context.CBound.there_var (E:=T) hb
-      exact hb1 }
-    { rw [← CaptureSet.proj_rename]; exact ih }
-  case cbound hb _ ih =>
-    apply cbound
-    { have hb1 := Context.CBound.there_var (E:=T) hb
-      exact hb1 }
-    { rw [← CaptureSet.proj_rename]; exact ih }
-  case ckind hb => apply ckind hb.there_var
-  case label hb hs =>
-    apply label
-    { have hb1 := Context.LBound.there_var (E:=T) hb
-      exact hb1 }
-    { apply hs.weaken }
-  case label_disj hb hd => apply label_disj hb.there_var hd
+  case empty => apply! empty
+  case union ha hb => apply! union
+  case ckind hb => apply! ckind hb.there_var
+  case label hb hl => apply label hb.there_var hl.weaken
+  case label_disj hb hd => apply! label_disj hb.there_var
+  case absurd => apply! absurd
+
 
 theorem TypedCont.weaken
   (h : TypedCont Γ E Cin t E' C0) :
@@ -185,38 +224,42 @@ theorem Cont.HasLabel.lweaken
     apply there_label; trivial
   case there_intercept => apply! there_intercept
 
+theorem ReachSet.lweaken
+  (hr : ReachSet Γ C R)
+  : ReachSet (Γ.label c S) C.weaken R.weaken := by
+  induction hr
+  case empty => constructor
+  case union ha hb => apply! union
+  case var hb hr ih =>
+    have hb1 := hb.there_label (c:=c) (S:=S)
+    apply var hb1
+    rw [← CaptureSet.proj_rename]; exact ih
+  case cinstr hb hr ih =>
+    have hb1 := hb.there_label (c:=c) (S:=S)
+    apply cinstr hb1
+    rw [← CaptureSet.proj_rename]; exact ih
+  case cbound hb hr ih =>
+    have hb1 := hb.there_label (c:=c) (S:=S)
+    apply cbound hb1
+    rw [← CaptureSet.proj_rename]; exact ih
+  case ckind hb =>
+    have hb1 := hb.there_label (c:=c) (S:=S)
+    apply ckind hb1
+  case label hb =>
+    have hb1 := hb.there_label (c':=c) (S':=S)
+    apply label hb1
+  case absurd he => apply! absurd
+
 theorem WellScoped.lweaken
   (h : WellScoped Γ cont Ct) :
   WellScoped (Γ.label c S) cont.weaken Ct.weaken := by
   induction h
-  case empty => simp [CaptureSet.weaken]; constructor
-  case union ih1 ih2 =>
-    simp [CaptureSet.weaken] at *
-    apply union <;> aesop
-  case singleton hb _ ih =>
-    apply singleton
-    { simp [FinFun.weaken]
-      have hb1 := Context.Bound.there_label (c:=c) (S:=S) hb
-      simp [CaptureSet.weaken, CaptureSet.rename] at hb1
-      exact hb1 }
-    { rw [← CaptureSet.proj_rename]; exact ih }
-  case csingleton hb _ ih =>
-    apply csingleton
-    { have hb1 := Context.CBound.there_label (c:=c) (S:=S) hb
-      exact hb1 }
-    { rw [← CaptureSet.proj_rename]; exact ih }
-  case cbound hb _ ih =>
-    apply cbound
-    { have hb1 := Context.CBound.there_label (c:=c) (S:=S) hb
-      exact hb1 }
-    { rw [← CaptureSet.proj_rename]; exact ih }
+  case empty => apply! empty
+  case union ha hb => apply! union
   case ckind hb => apply! ckind hb.there_label
-  case label hb hs =>
-    apply label
-    { have hb1 := Context.LBound.there_label (c':=c) (S':=S) hb
-      exact hb1 }
-    { apply hs.lweaken }
+  case label hb hl => apply label hb.there_label hl.lweaken
   case label_disj hb hd => apply! label_disj hb.there_label
+  case absurd => apply! absurd
 
 theorem TypedCont.lweaken
   (h : TypedCont Γ Cin E cont E' Ct) :
