Capless/Weakening/TypedCont/Type.lean
@@ -56,38 +56,42 @@ theorem Cont.HasLabel.tweaken
   case there_label => simp [Cont.tweaken]; apply there_label; aesop
   case there_intercept => apply! there_intercept
 
+theorem ReachSet.tweaken
+  (hr : ReachSet Γ C R)
+  : ReachSet (Γ.tvar b) C R := by
+  induction hr
+  case empty => constructor
+  case union ha hb => apply! union
+  case var hb hr ih =>
+    have hb1 := hb.there_tvar (b:=b)
+    apply var hb1
+    exact ih
+  case cinstr hb hr ih =>
+    have hb1 := hb.there_tvar (b':=b)
+    apply cinstr hb1
+    exact ih
+  case cbound hb hr ih =>
+    have hb1 := hb.there_tvar (b':=b)
+    apply cbound hb1
+    exact ih
+  case ckind hb =>
+    have hb1 := hb.there_tvar (b':=b)
+    apply ckind hb1
+  case label hb =>
+    have hb1 := hb.there_tvar (b:=b)
+    apply label hb1
+  case absurd he => apply! absurd
+
 theorem WellScoped.tweaken
   (h : WellScoped Γ cont Ct) :
   WellScoped (Γ.tvar b) cont.tweaken Ct := by
   induction h
-  case empty => constructor
-  case union ih1 ih2 => apply union <;> aesop
-  case singleton hb _ ih =>
-    apply singleton
-    { have hb1 := Context.Bound.there_tvar (b := b) hb
-      simp [CType.tweaken, CType.trename] at hb1
-      exact hb1 }
-    { exact ih }
-  case csingleton hb _ ih =>
-    apply csingleton
-    { have hb1 := Context.CBound.there_tvar (b' := b) hb
-      simp [CType.tweaken, CType.trename] at hb1
-      exact hb1 }
-    { exact ih }
-  case cbound hb _ ih =>
-    apply cbound
-    { have hb1 := Context.CBound.there_tvar (b' := b) hb
-      simp [CType.tweaken, CType.trename] at hb1
-      exact hb1 }
-    { exact ih }
-  case ckind hb => apply ckind hb.there_tvar
-  case label hb hs =>
-    apply label
-    { have hb1 := Context.LBound.there_tvar (b := b) hb
-      simp [CType.tweaken, CType.trename] at hb1
-      exact hb1 }
-    { apply hs.tweaken }
+  case empty => apply! empty
+  case union ha hb => apply! union
+  case ckind hb => apply! ckind hb.there_tvar
+  case label hb hl => apply label hb.there_tvar hl.tweaken
   case label_disj hb hd => apply! label_disj hb.there_tvar
+  case absurd => apply! absurd
 
 theorem TypedCont.tweaken
   (h : TypedCont Γ E Cin t E' C0) :
